share/steel/examples/pulse/parallel/GhostTaskQueue.fsti
@@ -71,3 +71,84 @@ val close_task_preserves_order (#a: Type)
 
 let pure_inv_queue #a (q: list a) (c: int) (l: mono_list a)
 = count_ongoing l = c /\ get_actual_queue l == q
+
+open Pulse.Lib.Pervasives
+
+module Lock = Pulse.Lib.SpinLock
+
+let one_quart = half_perm (half_perm full_perm)
+
+let own_res (#a: Type0) (r: ref (option a)) = (exists_ (fun v -> pts_to r #one_quart v))
+
+let unit_emp_stt_pure_pure a
+  = unit -> stt a emp (fun _ -> emp)
+
+let task_elem: Type u#1 = (
+  a: Type0 // return type of the computation
+  & r: ref (option a) // the reference where we put the result of the computation
+  & Lock.lock (own_res r)//(exists_ (fun v -> pts_to r half v ** (if None? v then pts_to r half v else emp)))
+  & (unit_emp_stt_pure_pure a)
+)
+
+val ghost_mono_ref (a: Type u#1): Type0
+
+val pts_to_ghost_queue (#a: Type) (r: ghost_mono_ref a) (l: mono_list a): vprop
+
+let three_quart = sum_perm (half_perm full_perm) (half_perm (half_perm full_perm))
+
+val certificate (r:ghost_mono_ref task_elem) (t: task_elem) (pos: nat): Type0
+
+val small_inv (r: ghost_mono_ref task_elem) (q: list task_elem) (c: int): vprop 
+
+// 1. enqueue task
+val spawn_task_ghost
+(r: ghost_mono_ref task_elem)
+(q: list task_elem) (c: int) (t: task_elem):
+stt_ghost (pos:nat & certificate r t pos) emp_inames
+(small_inv r q c ** pts_to t._2 #three_quart None)
+(fun _ -> small_inv r (t::q) c)
+
+// 2. pop task todo
+val pop_task_ghost
+(r: ghost_mono_ref task_elem)
+(t: task_elem)
+(q: list task_elem) (c: int) (t: task_elem):
+stt_ghost unit emp_inames
+(small_inv r (t::q) c)
+(fun () -> small_inv r q (c + 1) ** pts_to t._2 #three_quart None)
+
+// 3. conclude a task
+val conclude_task_ghost
+(#t: task_elem)
+(#pos: nat)
+(r: ghost_mono_ref task_elem)
+(q: list task_elem) (c: int)
+(x: t._1)
+(w: certificate r t pos):
+stt_ghost unit emp_inames
+(small_inv r q c ** pts_to t._2 #three_quart (Some x))
+(fun () -> small_inv r q (c - 1))
+
+
+val recall_certificate (#t: task_elem) (#pos: nat)
+           (r:ghost_mono_ref task_elem)
+           (v: mono_list task_elem)
+           (w:certificate r t pos)
+  : //TODO: SteelAtomicU
+ stt_ghost unit emp_inames
+                 (pts_to_ghost_queue r v)
+                 (fun _ -> pts_to_ghost_queue r v ** pure (task_in_queue t pos v))
+
+// in the end, we want
+// where's the other half permission to the thing?
+// in the handler
+// pool_done = get_actual_queue = [] and get_counter = 0
+// so, with half permission to the thing
+// and the certificate
+val get_Some_finished (#t: task_elem) (#pos: nat)
+  (r:ghost_mono_ref task_elem)
+  (w:certificate r t pos)
+: stt_ghost t._1 emp_inames
+(small_inv r [] 0)
+// that's the proof that it's finished
+(fun _ -> small_inv r [] 0)
